---
title: "Proof Practice"
categories:
  - mathforpaper
---
# Lemma 2.8

If $f: \mathbb{R}^d \rightarrow \mathbb{R}$ is convex and differentiable then,

$$
\text{for all} \; x, y \in \mathbb{R}^d, \quad f(x) \geq f(y) + \langle \nabla f(y), x - y \rangle
$$

*Proof*

$f: \mathbb{R}^d \rightarrow \mathbb{R}$ is convex

$\rightarrow$

$$
\forall x, y \in \mathbb{R}, \quad \text{for all} \; t \in [0, 1], \quad

f(tx + (1 - t)y) \leq t f(x) + (1 - t) f(y)
$$

$\rightarrow$

$$
\forall x, y \in \mathbb{R}, \quad \text{for all} \; t \in [0, 1], \quad

f(y + t(x - y)) \leq f(y) + t(f(x) - f(y))
$$

$\rightarrow$

$$
\forall x, y \in \mathbb{R}, \quad \text{for all} \; t \in (0, 1], \quad

\dfrac{f(y + t(x - y)) - f(y)}{t} \leq f(x) - f(y)
$$

$\rightarrow$

By differentiability,

$\text{for all} \; x, y \in \mathbb{R}^d, \quad$

$$
\begin{align*}
  \nabla_{x - y} f(y) = \lim_{t \to 0} \dfrac{f(y + t(x - y)) - f(y)}{t} = \lim_{t \to 0+} \dfrac{f(y + t(x - y)) - f(y)}{t} \leq \lim_{t \to 0+} \left( f(x) - f(y) \right) = f(x) - f(y)
\end{align*}
$$

$\rightarrow$

By definition of gradient,

$$
\forall x, y \in \mathbb{R}, \quad

\nabla_{x - y} f(y) = \langle \nabla f(y),\; x - y \rangle \leq f(x) - f(y)
$$

$\rightarrow$

$$
\forall x, y \in \mathbb{R}, \quad

f(x) \geq f(y) +  \langle \nabla f(y),\; x - y \rangle
$$

# Lemma 2.9

If $f: \mathbb{R}^d \rightarrow \mathbb{R}$ is convex and twice differentiable, for all $x \in \mathbb{R}^d$, for every eigenvalue $\lambda$ of $\nabla^2 f(x)$, we have $\lambda \geq 0$

*Proof*

$f: \mathbb{R}^d \rightarrow \mathbb{R}$ is convex and differentiable, by lemma 2.8,

$\rightarrow$

$\forall x, y \in \mathbb{R}^d$

$$
f(x) \geq f(y) + \langle \nabla f(y), \; x - y \rangle \\
f(y) \geq f(x) + \langle \nabla f(x), \; y - x \rangle
$$

$\rightarrow$

$\forall x, y \in \mathbb{R}^d$

$$
f(x) + f(y) \geq f(x) + f(y) + \langle \nabla f(y), \; x - y \rangle +  \langle \nabla f(x), \; y - x \rangle
$$

$\rightarrow$

$\forall x, y \in \mathbb{R}^d$

$$
\begin{align*}
0 & \geq \langle \nabla f(y), \; x - y \rangle +  \langle \nabla f(x), \; y - x \rangle \\
&= \nabla f(y)^{\top} (x - y) + \nabla f(x)^{\top} (y - x) \\
&= - (\nabla f(y)^{\top} - \nabla f(x)^{\top}) (y - x) \\
&= - (\nabla f(y) - \nabla f(x))^{\top} (y - x) \\
&= - \langle \nabla f(y) - \nabla f(x), \; y - x \rangle \\
\end{align*}
$$

$\rightarrow$

$\forall x, y \in \mathbb{R}^d$

$$
0 \leq \langle \nabla f(y) - \nabla f(x), \; y - x \rangle
$$

$\rightarrow$

$\forall x, y \in \mathbb{R}^d, \; \forall t \in \mathbb{R} \setminus \{0\}, \; \forall v = \dfrac{y - x}{t} \in \mathbb{R}^d$

$$
\begin{align*}
0 &\leq \langle \nabla f(y) - \nabla f(x), \; y - x \rangle \\
&= \langle \nabla f(x + tv) - \nabla f(x), \; tv \rangle \\
\end{align*}
$$

$\rightarrow$

$\forall x, v\in \mathbb{R}^d, \; \forall t \in \mathbb{R} \setminus \{0\}$

$$
\begin{align*}
0 &\leq \dfrac{1}{t^2} \langle \nabla f(x + tv) - \nabla f(x), \; tv \rangle \\
&= \left\langle \dfrac{\nabla f(x + tv) - \nabla f(x)}{t}, \; v \right\rangle \\
\end{align*}
$$

$\rightarrow$

$\forall x, v\in \mathbb{R}^d, \; \forall t \in \mathbb{R} \setminus \{0\}$

$$
\begin{align*}
0 &\leq \lim_{t \to 0} \left\langle \dfrac{\nabla f(x + tv) - \nabla f(x)}{t}, \; v \right\rangle \\
&= \left\langle \lim_{t \to 0} \dfrac{\nabla f(x + tv) - \nabla f(x)}{t}, \; v \right\rangle \\
&= \left\langle \nabla^2 f(x) v, \; v \right\rangle \\
\end{align*}
$$

# Lemma 2.12

Let $f: \mathbb{R}^d \rightarrow \mathbb{R}$, and $\mu > 0$. The function $f$ is $\mu$-strongly convex if and only if $g$ is convex if and only if there exists a convex function $g: \mathbb{R}^d \rightarrow \mathbb{R}$ such that $f(x) = g(x) + \dfrac{\mu}{2} \vert\vert x \vert\vert^2$.

*Proof*

$$
\begin{align*}
& tg(x) + (1 - t)g(y) - g(tx + (1 - t)y) \\
&= t \left\{ f(x) - \dfrac{\mu}{2} \vert\vert x \vert\vert^2 \right\} + (1 - t) \left\{ f(y) - \dfrac{\mu}{2} \vert\vert y \vert\vert^2 \right\} - \left\{ f(tx + (1 - t)y) - \dfrac{\mu}{2} \vert\vert tx + (1 - t)y \vert\vert^2 \right\} \\
&= tf(x) + (1 - t)f(y) - f(tx + (1 - t)y) - \dfrac{\mu}{2} \left\{ t \vert\vert x \vert\vert^2 + (1 - t) \vert\vert y \vert\vert^2 - \vert\vert tx + (1 - t)y \vert\vert^2\right\} \\
&= tf(x) + (1 - t)f(y) - f(tx + (1 - t)y) - \mu \dfrac{t(1 - t)}{2} \vert\vert x - y \vert\vert^2 \geq 0
\end{align*}
$$

since

$$
\begin{align*}
&\left\{ t \vert\vert x \vert\vert^2 + (1 - t) \vert\vert y \vert\vert^2 - \vert\vert tx + (1 - t)y \vert\vert^2\right\} \\
&=
\end{align*}
$$